Lots of edits, do_eval/end_eval is working
So, it looks like the invariants are basically right so that
adding an eval generation with do_eval and exiting it with
reset_env_generation, and saving an env with Denv all work
out ok.

The main missing thing is that source Eval also saves the
final env and returns it, which will require some stub code
to make it work.

compiler/backend/proofs/source_to_flatProofScript.sml
@@ -500,6 +500,7 @@ Triviality v_rel_weakening2:
     ∀gc. genv.c ⊑ genv'.c ∧ genv.tys ⊑ genv'.tys ∧ genv.v = genv'.v ⇒
     global_env_inv genv' comp_map shadowers env)
 Proof
+  ho_match_mp_tac v_rel_ind >>
   srw_tac[][v_rel_eqns] >>
   fs [SUBMAP_FLOOKUP_EQN]
   >- fs [LIST_REL_EL_EQN]
@@ -1819,15 +1820,19 @@ Definition orac_rel_def:
     | _ => F)
 End
 
+Definition src_orac_next_cfg_inner_def:
+  src_orac_next_cfg_inner interp orac_0 = case (interp, orac_0) of
+    | (SOME i, (env_id, state_v, decs)) =>
+      (case i.decode_state state_v of
+        | SOME (c, x) => SOME c
+        | _ => NONE
+      )
+    | _ => NONE
+End
+
 Definition src_orac_next_cfg_def:
-  src_orac_next_cfg interp eval_state = case (interp, eval_state) of
-    | (SOME i, SOME (EvalOracle s)) =>
-    (case s.oracle 0 of (env_id, state_v, decs) =>
-        (case i.decode_state state_v of
-          | SOME (c, x) => SOME c
-          | _ => NONE
-        )
-    )
+  src_orac_next_cfg interp eval_state = case eval_state of
+    | SOME (EvalOracle s) => src_orac_next_cfg_inner interp (s.oracle 0)
     | _ => NONE
 End
 
@@ -1886,14 +1891,12 @@ End
 (* the compiler state in the oracle represents a future compilation, which
    will already have this generation stored *)
 Definition env_gen_end_rel_def:
-  env_gen_end_rel gen interp eval_state = (case eval_state of
-    | NONE => T
-    | SOME (EvalOracle s) =>
-        ?c gen_final. src_orac_next_cfg interp eval_state = SOME c ∧
+  env_gen_end_rel gen interp eval_state =
+    (case src_orac_next_cfg interp eval_state of
+      | SOME c => ? gen_final.
         lookup gen.generation c.envs.env_gens = SOME gen_final /\
         subspt gen.envs gen_final
-    | _ => F
-  )
+      | NONE => T)
 End
 
 (* indexes and ranges: the source-to-flat compiler allocates names in order.
@@ -1943,6 +1946,36 @@ Definition invariant_def:
     env_gen_rel gen s.eval_state ∧
     fin_idx_match (LENGTH s_i1.globals) (src_orac_next_cfg interp s.eval_state)
 End
+
+(* this relation holds over any successful evaluate or evaluate_decs
+   - the generation stack is a call stack, and returns to where it was
+*)
+Definition orac_forward_rel_def:
+  orac_forward_rel es1 es2 ⇔
+    (case es1 of
+      | SOME (EvalOracle s1) => ?s2. es2 = SOME (EvalOracle s2) /\
+        s2.generation = s1.generation /\
+        LENGTH s1.envs <= LENGTH s2.envs /\
+        (!i. i < s1.generation ==> EL i s2.envs = EL i s1.envs)
+      | _ => T)
+End
+
+Theorem orac_forward_rel_trans:
+  orac_forward_rel es1 es2 /\ orac_forward_rel es2 es3 ==>
+  orac_forward_rel es1 es3
+Proof
+  fs [orac_forward_rel_def]
+  \\ every_case_tac \\ fs []
+  \\ rw []
+QED
+
+Theorem orac_forward_rel_refl[simp]:
+  orac_forward_rel es1 es1
+Proof
+  fs [orac_forward_rel_def]
+  \\ every_case_tac \\ fs []
+QED
+
 
 Theorem can_pmatch_all_IMP_pmatch_rows:
   can_pmatch_all env.c st.refs (MAP FST pes) v /\
@@ -2042,7 +2075,7 @@ QED
 
 Theorem compile_decs_idx_prev:
   !t n next env envs ds n' next' env' envs' ds_i1.
-    compile_decs t n next env envs ds = (n', next',env',envs',ds_i1)
+    compile_decs t n next env envs ds = (n', next', env', envs', ds_i1)
     ⇒
     idx_prev next next'
 Proof
@@ -2065,6 +2098,22 @@ Proof
   \\ rw []
   \\ simp []
 QED
+
+Theorem compile_decs_generation:
+  !t n next env envs ds n' next' env' envs' ds_i1.
+    compile_decs t n next env envs ds = (n', next', env', envs', ds_i1)
+    ⇒
+    envs'.generation = envs.generation
+Proof
+  ho_match_mp_tac compile_decs_ind >>
+  rw [compile_decs_def, idx_prev_def] >>
+  rw [] >>
+  pairarg_tac >>
+  fs [] >>
+  pairarg_tac >>
+  fs []
+QED
+
 
 Triviality v_rel_eqns_non_global =
   v_rel_eqns |> BODY_CONJUNCTS
@@ -2223,34 +2272,6 @@ Proof
   simp [ALL_DISJOINT_DEF, EVERY_EL, EXTENSION]
   \\ metis_tac []
 QED
-
-(* FIXME: previous version assumed oracle state could be used to
-   pick a fin_idx, that's more complicated now
-
-Theorem idx_range_rel_v_REPLICATE_NONE:
-  idx_range_rel genv nts nes eval_mode (idx, end_idx, others) ∧
-  eval_idx_match_len eval_mode (LENGTH genv.v) ∧
-  n + idx.vidx <= end_idx.vidx
-  ==>
-  ?pre post. genv.v = pre ++ REPLICATE n NONE ++ post ∧
-    LENGTH pre = idx.vidx
-Proof
-  rw [idx_range_rel_def, eval_idx_match_len_def]
-  \\ qexists_tac `TAKE idx.vidx genv.v`
-  \\ qexists_tac `DROP (idx.vidx + n) genv.v`
-  \\ fs [idx_prev_def]
-  \\ qsuff_tac `!i. idx.vidx <= i /\ i < n + idx.vidx ==> EL i genv.v = NONE`
-  >- (
-    REWRITE_TAC [GSYM LIST_REL_eq, LIST_REL_EL_EQN]
-    \\ simp [EL_APPEND_IF]
-    \\ rw [] \\ rw []
-    \\ simp [EL_TAKE, EL_REPLICATE, EL_DROP]
-  )
-  \\ rw []
-  \\ qspecl_then [`(i, Idx_Var)`, `0`] drule ALL_DISJOINT_elem
-  \\ simp [idx_block_def]
-QED
-*)
 
 Theorem subglobals_NONE:
   subglobals (REPLICATE n NONE) g <=> n <= LENGTH g
@@ -2548,639 +2569,6 @@ Proof
   \\ simp [FLOOKUP_FUNION]
 QED
 
-(*
-FIXME eval_mode update
-Theorem invariant_begin_eval:
-  invariant interp gen genv (idx, end_idx, other) st st' ⇒
-  st'.eval_mode = Eval e ∧ e.compiler_state = fin_idx ∧
-  idx_prev fin_idx new_end_idx ∧ idx_prev new_end_idx new_fin_idx ⇒
-  ? genv'. invariant interp gen genv' (fin_idx, new_end_idx, idx_block idx end_idx ∪ other)
-    st (st' with <| eval_mode := Eval (e with compiler_state := new_fin_idx);
-            globals := st'.globals ++
-                REPLICATE (new_fin_idx.vidx - fin_idx.vidx) NONE |>) ∧
-  genv'.c = genv.c ∧ genv'.tys = genv.tys ∧ subglobals genv.v genv'.v
-Proof
-  rw [invariant_def]
-  \\ qabbrev_tac `genv' = genv with v := genv.v ++
-        REPLICATE (new_fin_idx.vidx - e.compiler_state.vidx) NONE`
-  \\ `subglobals genv.v genv'.v`
-    by fs [markerTheory.Abbrev_def, subglobals_def, EL_APPEND1]
-  \\ qexists_tac `genv'`
-  \\ fs [idx_range_rel_def, s_rel_cases, idx_prev_def, markerTheory.Abbrev_def]
-  \\ rveq \\ fs [] \\ rfs []
-  \\ conj_tac
-  >- (
-    drule_then irule LIST_REL_sv_rel_weak
-    \\ simp []
-  )
-  \\ csimp [EL_APPEND_IF, bool_case_eq, EL_REPLICATE]
-  \\ qspecl_then [`0`, `2`] drule ALL_DISJOINT_MOVE
-  \\ disch_then (qspec_then `idx_block idx end_idx` mp_tac)
-  \\ rw [LUPDATE_compute]
-  \\ qspecl_then [`1`, `0`] drule ALL_DISJOINT_MOVE
-  \\ disch_then (qspec_then `idx_block fin_idx new_end_idx` mp_tac)
-  \\ simp [LUPDATE_compute]
-  \\ impl_tac
-  >- (
-    simp [idx_block_def, idx_final_block_def]
-    \\ simp [SUBSET_DEF, PULL_EXISTS]
-  )
-  \\ rw []
-  \\ drule_then irule ALL_DISJOINT_SUBSETS
-  \\ simp []
-  \\ simp [SUBSET_DEF, PULL_EXISTS]
-  \\ rw [idx_final_block_def, idx_block_def]
-QED
-*)
-
-Theorem invariant_end_eval:
-  invariant interp gen genv (x, end_idx1, idx_block idx end_idx ∪ other) st st' ∧
-  invariant interp gen prev_genv (idx, end_idx, other) prev_st prev_st' ∧
-  idx_prev end_idx end_idx1 ⇒
-  invariant interp gen genv (idx, end_idx, other) st st'
-Proof
-  rw [invariant_def]
-  \\ fs [idx_range_rel_def]
-  \\ TRY asm_exists_tac
-  \\ fsrw_tac [SATISFY_ss] [idx_prev_trans]
-  \\ drule (Q.SPECL [`2`, `0`, `mv_set`, `[_; _; mv_set ∪ other; _]`]
-        ALL_DISJOINT_MOVE)
-  \\ rw [LUPDATE_compute]
-  \\ drule_then irule ALL_DISJOINT_SUBSETS
-  \\ simp []
-  \\ simp [SUBSET_DEF, PULL_EXISTS]
-  \\ imp_res_tac (Q.SPECL [`x`, `2`] ALL_DISJOINT_elem)
-  \\ fs []
-QED
-
-Theorem alloc_tags1_imp:
-  ! ctors ns spt tag_list.
-  alloc_tags1 ctors = (ns, spt, tag_list) ∧
-  ALL_DISTINCT (MAP FST ctors) ==>
-  ? cn_tags.
-  ns = alist_to_ns (MAP (\(cn, tag, arity). (cn, tag)) cn_tags) ∧
-  set (MAP SND cn_tags) = {(tag, arity) |
-    ∃max. lookup arity spt = SOME max ∧ tag < max} ∧
-  tag_list = MAP SND cn_tags ∧
-  ALL_DISTINCT tag_list ∧
-  LIST_REL (\(cn, ts) (cn', _, arity). cn = cn' ∧ arity = LENGTH ts)
-    ctors cn_tags ∧
-  MAP FST ctors = MAP FST cn_tags
-Proof
-  ho_match_mp_tac alloc_tags1_ind
-  \\ simp [alloc_tags1_def]
-  \\ rw []
-  \\ rpt (pairarg_tac \\ fs [])
-  \\ rveq \\ fs []
-  \\ simp [PULL_EXISTS, EXISTS_PROD, lookup_def]
-  \\ qexists_tac `cn_tags`
-  \\ fs [lookup_inc_def, option_case_eq] \\ rveq \\ fs []
-  \\ simp [EVERY_MEM, MEM_MAP, FORALL_PROD, EXISTS_PROD]
-  \\ simp [lookup_insert, EXTENSION]
-  \\ rw [] \\ EQ_TAC \\ rw []
-  \\ rw [] \\ fs []
-  \\ fs [bool_case_eq, Q.ISPEC `SOME v` EQ_SYM_EQ]
-QED
-
-(* FIXME also in flat_pattern *)
-Theorem ALOOKUP_MAP_3:
-  (!x. MEM x xs ==> FST (f x) = FST x) ==>
-  ALOOKUP (MAP f xs) x = OPTION_MAP (\y. SND (f (x, y))) (ALOOKUP xs x)
-Proof
-  Induct_on `xs` \\ rw []
-  \\ fs [DISJ_IMP_THM, FORALL_AND_THM]
-  \\ Cases_on `f h`
-  \\ Cases_on `h`
-  \\ rw []
-  \\ fs []
-QED
-
-(* not sure why this is broken ATM
-Theorem alloc_tags_invariant:
-  alloc_tags idx.tidx (ctors : (string # ast_t list) list) = (ns, cids) ∧
-  invariant interp gen genv (idx, end_idx, os) st st' ∧
-  global_env_inv genv comp_map {} env ∧
-  ALL_DISTINCT (MAP FST ctors) ∧
-  idx.tidx + 1 <= end_idx.tidx
-  ⇒
-  ?genv'.
-  genv.c ⊑ genv'.c ∧
-  genv.tys ⊑ genv'.tys ∧
-  genv'.v = genv.v ∧
-  invariant interp gen genv' (idx with tidx := idx.tidx + 1, end_idx, os)
-    (st with next_type_stamp := st.next_type_stamp + 1)
-    (st' with c updated_by $UNION {((idx',SOME idx.tidx),arity) |
-                       (∃max. lookup arity cids = SOME max ∧ idx' < max)}) ∧
-  (let build_env = <| c := alist_to_ns
-        (REVERSE (build_constrs st.next_type_stamp ctors)); v := nsEmpty |> in
-   global_env_inv genv' <| c := ns; v := nsEmpty |> {} build_env ∧
-   env_domain_eq <|c := ns; v := nsEmpty|> build_env)
-Proof
-  rw [invariant_def]
-  \\ fs [s_rel_cases]
-  \\ fs [alloc_tags_def]
-  \\ rpt (pairarg_tac \\ fs [])
-  \\ rveq \\ fs []
-  \\ Cases_on `ctors = []`
-  >- (
-    fs [alloc_tags1_def] \\ rveq \\ fs []
-    \\ qexists_tac `genv`
-    \\ simp [lookup_def, build_constrs_def, v_rel_cases, env_domain_eq_def]
-    \\ fs [idx_range_rel_def]
-    \\ asm_exists_tac
-    \\ simp []
-    \\ drule_then irule ALL_DISJOINT_SUBSETS
-    \\ simp []
-    \\ simp [SUBSET_DEF, idx_block_def]
-    \\ rw []
-  )
-  \\ drule alloc_tags1_imp
-  \\ rw []
-  \\ qexists_tac `genv with <| c := FUNION genv.c (alist_to_fmap
-        (MAP (\(cn, tag, arity). (((tag, SOME idx.tidx), arity),
-            TypeStamp cn st.next_type_stamp)) cn_tags));
-        tys := FUNION genv.tys (alist_to_fmap [(idx.tidx, MAP SND cn_tags)])
-    |>`
-  \\ rw [SUBMAP_FUNION_ID]
-  >- (
-    drule_then irule genv_c_ok_extend
-    \\ rw [FORALL_PROD]
-    \\ imp_res_tac ALOOKUP_MEM
-    \\ fs [MEM_MAP, EXISTS_PROD] \\ rveq \\ fs []
-    \\ simp [same_type_def, ctor_same_type_def]
-    \\ rveq \\ fs []
-    \\ imp_res_tac alistTheory.ALOOKUP_ALL_DISTINCT_MEM
-    \\ fs []
-    \\ TRY strip_tac
-    \\ rveq \\ fs []
-    \\ fs [idx_range_rel_def]
-    \\ rfs [FRANGE_FLOOKUP]
-    \\ qspecl_then [`(i,Idx_Type)`, `0`] drule ALL_DISJOINT_elem
-    \\ simp [idx_block_def]
-    \\ qexists_tac `idx.tidx`
-    \\ simp [FDOM_FLOOKUP]
-    \\ metis_tac []
-  )
-  >- (
-    irule genv_c_tys_ok_extend
-    \\ simp [genv_c_tys_ok_def]
-    \\ conj_tac
-    >- (
-      fs [idx_range_rel_def, genv_c_tys_ok_def]
-      \\ qspecl_then [`(i,Idx_Type)`, `0`] drule ALL_DISJOINT_elem
-      \\ simp []
-      \\ disch_then (qspec_then `idx.tidx` mp_tac)
-      \\ simp [idx_block_def]
-    )
-    \\ simp [genv_c_tys_ok_def, MEM_MAP, EXISTS_PROD, PULL_EXISTS]
-    \\ simp [FLOOKUP_UPDATE, MEM_MAP, EXISTS_PROD]
-    \\ metis_tac []
-  )
-  >- (
-    drule_then irule LIST_REL_sv_rel_weak
-    \\ simp [subglobals_refl, SUBMAP_FUNION_ID]
-  )
-  >- (
-    fs [EXTENSION, FORALL_PROD, MEM_MAP, EXISTS_PROD]
-    \\ metis_tac []
-  )
-  >- (
-    fs [idx_range_rel_def]
-    \\ asm_exists_tac
-    \\ rw []
-    \\ fs [FRANGE_FLOOKUP, FLOOKUP_FUNION, option_case_eq, FLOOKUP_UPDATE]
-    \\ TRY (CCONTR_TAC \\ fs [] \\ imp_res_tac ALOOKUP_MEM
-      \\ fs [MEM_MAP, EXISTS_PROD] \\ NO_TAC)
-    \\ drule_then irule (Q.SPECL [`0`, `3`] ALL_DISJOINT_MOVE)
-    \\ simp [LUPDATE_compute]
-    \\ qexists_tac `{(idx.tidx, Idx_Type)}`
-    \\ simp [EXTENSION, FORALL_PROD, idx_types_FORALL, idx_block_def]
-    \\ simp [MEM_MAP, EXISTS_PROD, PULL_EXISTS]
-    \\ rw [] \\ EQ_TAC \\ rw []
-    \\ fs [NOT_NIL_EQ_LENGTH_NOT_0, quantHeuristicsTheory.LIST_LENGTH_2]
-    \\ rveq \\ fs [EXISTS_PROD]
-    \\ metis_tac []
-  )
-  >- (
-    simp [build_constrs_def]
-    \\ simp [Once v_rel_cases]
-    \\ rw [nsLookup_alist_to_ns_some]
-    \\ imp_res_tac ALOOKUP_MEM
-    \\ fs [MEM_MAP, EXISTS_PROD] \\ rveq \\ fs []
-    \\ simp [MAP_MAP_o, o_DEF, ELIM_UNCURRY]
-    \\ drule_then drule LIST_REL_MEM_IMP
-    \\ rw [EXISTS_PROD]
-    \\ imp_res_tac alistTheory.ALOOKUP_ALL_DISTINCT_MEM
-    \\ simp [ALOOKUP_MAP_3, FLOOKUP_FUNION]
-    \\ simp [option_case_eq, ALOOKUP_MAP_3]
-    \\ rfs [idx_range_rel_def, FLOOKUP_UPDATE]
-    \\ qspecl_then [`(i,Idx_Type)`, `0`] drule ALL_DISJOINT_elem
-    \\ simp []
-    \\ disch_then (qspec_then `idx.tidx` mp_tac)
-    \\ simp [idx_block_def, flookup_thm]
-    \\ rw []
-    \\ irule alistTheory.ALOOKUP_ALL_DISTINCT_MEM
-    \\ simp [MEM_MAP, EXISTS_PROD]
-    \\ simp [MAP_MAP_o, o_DEF]
-    \\ simp [GSYM MAP_MAP_o |> REWRITE_RULE [o_DEF] |> Q.SPEC `f`
-                |> Q.ISPEC `SND`]
-    \\ irule ALL_DISTINCT_MAP_INJ
-    \\ simp [FORALL_PROD]
-  )
-  >- (
-    simp [env_domain_eq_def]
-    \\ simp [MAP_MAP_o, o_DEF, build_constrs_def, MAP_REVERSE, ELIM_UNCURRY]
-    \\ simp [GSYM MAP_MAP_o |> REWRITE_RULE [o_DEF] |> Q.SPEC `f`
-                |> Q.ISPEC `FST`]
-  )
-QED
-*)
-
-val nsAppend_foldl' = Q.prove (
-  `!l ns ns'.
-   nsAppend (FOLDL (λns (l,cids). nsAppend l ns) ns' l) ns
-   =
-   FOLDL (λns (l,cids). nsAppend l ns) (nsAppend ns' ns) l`,
-  Induct_on `l` >>
-  rw [] >>
-  PairCases_on `h` >>
-  rw []);
-
-val nsAppend_foldl = Q.prove (
-  `!l ns.
-   FOLDL (λns (l,cids). nsAppend l ns) ns l
-   =
-   nsAppend (FOLDL (λns (l,cids). nsAppend l ns) nsEmpty l) ns`,
-  metis_tac [nsAppend_foldl', nsAppend_nsEmpty]);
-
-val build_tdefs_no_mod = Q.prove (
-  `!idx tdefs. nsDomMod (build_tdefs idx tdefs) = {[]}`,
-  Induct_on `tdefs` >>
-  rw [build_tdefs_def] >>
-  PairCases_on `h` >>
-  rw [build_tdefs_def] >>
-  pop_assum (qspec_then `idx+1` mp_tac) >>
-  rw [nsDomMod_nsAppend_flat]);
-
-val extend_env_v_empty =
-``extend_env <| c := c; v := nsEmpty |> <| c := c'; v := nsEmpty |>``
-  |> SIMP_CONV (srw_ss ()) [extend_env_def]
-
-val extend_dec_env_v_empty =
-``extend_dec_env <| c := c; v := nsEmpty |> <| c := c'; v := nsEmpty |>``
-  |> SIMP_CONV (srw_ss ()) [extend_dec_env_def]
-
-Theorem compile_env_exp:
-  global_env_inv genv comp_map ∅ env ==>
-  ?v. evaluate env' s [compile_env_exp t comp_map] = (s, Rval [v])
-  /\ v_rel genv (Env env) v
-Proof
-  cheat
-QED
-
-Theorem nsLookup_nsBind_If:
-  nsLookup (nsBind n v e) nm = (if nm = Short n then SOME v else nsLookup e nm)
-Proof
-  Cases_on `e`
-  \\ Cases_on `nm`
-  \\ simp [namespaceTheory.nsBind_def, namespaceTheory.nsLookup_def]
-  \\ simp [EQ_SYM_EQ]
-QED
-
-Theorem invariant_IMP_s_rel:
-  invariant interp gen genv idx st st' ==> s_rel genv st st'
-Proof
-  simp [invariant_def]
-QED
-
-Theorem invariant_to_st_refs:
-  invariant interp gen genv idx st st' ==>
-  LIST_REL (sv_rel genv) st.refs st'.refs
-Proof
-  simp [invariant_def, s_rel_cases]
-QED
-
-Definition abort_def:
-  abort r <=> (case r of Rerr (Rabort a) => T
-    | _ => F)
-End
-
-Triviality not_abort_IMP_cases:
-  (~ abort r ==> P) ==>
-  ((?a. r = Rerr (Rabort a)) \/ (~ abort r /\ P))
-Proof
-  simp [abort_def] \\ every_case_tac \\ simp []
-QED
-
-Theorem abort_simps[simp]:
-  abort (Rerr (Rabort a)) = T /\
-  abort (Rerr (Rraise e)) = F /\
-  abort (Rval v) = F
-Proof
-  simp [abort_def]
-QED
-
-Definition Case_def:
-  Case X <=> T
-End
-
-Theorem elim_Case:
-  (Case X /\ Y) = Y /\
-  (Case X ==> Y) = Y
-Proof
-  simp [Case_def]
-QED
-
-fun is_app_case t = is_comb t andalso same_const ``Case`` (rator t)
-
-fun setup (q : term quotation, t : tactic) = let
-    val the_concl = Parse.typedTerm q bool
-    val t2 = (t \\ rpt (pop_assum mp_tac))
-    val (goals, validation) = t2 ([], the_concl)
-    fun get_goal q = first (can (rename [q])) goals |> snd
-    fun init thms st = if null (fst st) andalso aconv (snd st) the_concl
-      then ((K (goals, validation)) \\ TRY (MAP_FIRST ACCEPT_TAC thms)) st
-      else failwith "setup tactic: mismatching starting state"
-    val cases = map (find_terms is_app_case o snd) goals
-  in {get_goal = get_goal, concl = fn () => the_concl,
-    cases = cases, init = (init : thm list -> tactic),
-    all_goals = fn () => map snd goals} end
-
-val compile_correct_setup = setup (`
-  (∀ ^s env es s' r genv comp_map env_i1 ^s_i1 es_i1 locals t ts gen idxs.
-    evaluate$evaluate s env es = (s', r) ∧
-    Case es ∧
-    invariant interp gen genv idxs s s_i1 ∧
-    env_all_rel genv comp_map env env_i1 locals ∧
-    LENGTH ts = LENGTH locals ∧
-    r ≠ Rerr (Rabort Rtype_error) ∧
-    es_i1 = compile_exps t (comp_map with v := bind_locals ts locals comp_map.v) es
-    ⇒
-    ?s'_i1 r_i1 genv'.
-    flatSem$evaluate env_i1 s_i1 es_i1 = (s'_i1, r_i1) ∧
-    result_rel (LIST_REL o v_rel) genv' r r_i1 ∧
-    s_rel genv' s' s'_i1 ∧
-    (~ abort r ⇒
-      invariant interp gen genv' idxs s' s'_i1 ∧
-      genv.c ⊑ genv'.c ∧
-      genv.tys ⊑ genv'.tys ∧
-      subglobals genv.v genv'.v)
-  ) ∧
-  (∀ ^s env v pes err_v genv comp_map s' r env_i1 ^s_i1 v_i1 pes_i1
-         err_v_i1 locals t ts gen idxs.
-    evaluate$evaluate_match s env v pes err_v = (s', r) ∧
-    Case pes ∧
-    invariant interp gen genv idxs s s_i1 ∧
-    env_all_rel genv comp_map env env_i1 locals ∧
-    v_rel genv v v_i1 ∧
-    LENGTH ts = LENGTH locals ∧
-    r ≠ Rerr (Rabort Rtype_error) ∧
-    pes_i1 = compile_pes t (comp_map with v := bind_locals ts locals comp_map.v) pes ∧
-    pmatch_rows pes_i1 s_i1 v_i1 <> Match_type_error ∧
-    v_rel genv err_v err_v_i1
-    ⇒
-    ?s'_i1 r_i1 genv'.
-    flatProps$evaluate_match env_i1 s_i1 v_i1 pes_i1 err_v_i1 = (s'_i1, r_i1) ∧
-    result_rel (LIST_REL o v_rel) genv' r r_i1 ∧
-    s_rel genv' s' s'_i1 ∧
-    (~ abort r ⇒
-      invariant interp gen genv' idxs s' s'_i1 ∧
-      genv.c ⊑ genv'.c ∧
-      genv.tys ⊑ genv'.tys ∧
-      subglobals genv.v genv'.v)
-  ) ∧
-  (∀ ^s env ds s' r path t idx end_idx os comp_map ^s_i1 idx'
-        comp_map' ds_i1 t' genv gen gen'.
-    evaluate$evaluate_decs s env ds = (s',r) ∧
-    Case ds ∧
-    invariant interp gen genv (idx, end_idx, os) s s_i1 ∧
-    source_to_flat$compile_decs path t idx comp_map gen ds =
-        (t', idx', comp_map', gen', ds_i1) ∧
-    env_gen_end_rel gen' interp s.eval_state ∧
-    r ≠ Rerr (Rabort Rtype_error) ∧
-    global_env_inv genv comp_map {} env ∧
-    idx_prev idx' end_idx
-    ⇒
-    ? ^s1_i1 genv' r_i1.
-    flatSem$evaluate_decs s_i1 ds_i1 = (s1_i1,r_i1) ∧
-    s_rel genv' s' s1_i1 ∧
-    (~ abort r ⇒
-      invariant interp gen' genv' (idx', end_idx, os) s' s1_i1 ∧
-      genv.c ⊑ genv'.c ∧
-      genv.tys ⊑ genv'.tys ∧
-      subglobals genv.v genv'.v
-    ) ∧
-    (!env'.
-      r = Rval env'
-      ⇒
-      r_i1 = NONE ∧
-      env_domain_eq comp_map' env' ∧
-      global_env_inv genv' comp_map' {} env') ∧
-    (!err.
-      r = Rerr err
-      ⇒
-      ?err_i1.
-        r_i1 = SOME err_i1 ∧
-        result_rel (\a b (c:'a). T) genv' (Rerr err) (Rerr err_i1))
-  )
-  `,
-  ho_match_mp_tac terminationTheory.full_evaluate_ind
-  \\ rw [terminationTheory.full_evaluate_def, flat_evaluate_def,
-    compile_exp_def, compile_decs_def]
-  \\ imp_res_tac invariant_IMP_s_rel
-  \\ fs [result_rel_eqns, v_rel_eqns_non_global, elim_Case]
-)
-
-(*
-  #all_goals compile_correct_setup ()
-*)
-
-Triviality compile_correct_seq:
-  ^(#get_goal compile_correct_setup `Case (_ :: _ :: _)`)
-Proof
-  rw []
-  \\ fs [pair_case_eq] \\ fs []
-  \\ first_x_assum (drule_then (drule_then drule))
-  \\ disch_then (qspec_then ‘t’ mp_tac)
-  \\ reverse (fs [result_case_eq])
-  >- (
-    rw []
-    \\ fs [result_rel_cases]
-    \\ asm_exists_tac \\ simp []
-  )
-  \\ fs [pair_case_eq]
-  \\ rveq \\ fs []
-  \\ rw []
-  \\ fs [result_rel_cases]
-  \\ rveq \\ fs []
-  \\ drule_then drule env_all_rel_weak
-  \\ rw []
-  \\ first_x_assum (drule_then (drule_then drule))
-  \\ disch_then (qspec_then ‘t’ mp_tac)
-  \\ simp []
-  \\ impl_tac >- (CCONTR_TAC >> fs [])
-  \\ imp_res_tac evaluate_sing \\ fs [] \\ rveq \\ fs []
-  \\ rw [] \\ fs [] \\ rveq \\ fs []
-  \\ metis_tac [v_rel_weak, SUBMAP_TRANS, subglobals_trans]
-QED
-
-Triviality compile_correct_Raise:
-  ^(#get_goal compile_correct_setup `Case [Raise _]`)
-Proof
-  rw []
-  \\ fs [pair_case_eq]
-  \\ rveq \\ fs []
-  \\ first_x_assum (drule_then (drule_then drule))
-  \\ disch_then (qspec_then ‘t’ mp_tac)
-  \\ simp []
-  \\ impl_tac >- (CCONTR_TAC \\ fs [])
-  \\ rw []
-  \\ fs [result_rel_cases] \\ rveq \\ fs [] \\ rveq \\ fs []
-  \\ imp_res_tac evaluatePropsTheory.evaluate_sing
-  \\ imp_res_tac evaluate_sing
-  \\ rveq \\ fs []
-  \\ asm_exists_tac \\ simp []
-QED
-
-Triviality compile_correct_Handle:
-  ^(#get_goal compile_correct_setup `Case [Handle _ _]`)
-Proof
-  rw []
-  \\ fs [pair_case_eq] \\ fs []
-  \\ first_x_assum (drule_then (drule_then drule))
-  \\ disch_then (qspec_then ‘t’ mp_tac)
-  \\ simp []
-  \\ impl_tac >- (CCONTR_TAC \\ fs [])
-  \\ rw []
-  \\ imp_res_tac result_rel_imp \\ fs [] \\ rveq \\ fs []
-  \\ TRY (asm_exists_tac \\ simp [])
-  \\ fs [bool_case_eq, Q.ISPEC `(a, b)` EQ_SYM_EQ]
-  \\ drule_then drule env_all_rel_weak
-  \\ rw []
-  \\ first_x_assum (drule_then drule)
-  \\ rpt (disch_then drule)
-  \\ disch_then (first_assum o mp_then (Pat `v_rel`) mp_tac)
-  \\ disch_then (qspec_then ‘t’ mp_tac)
-  \\ DEP_REWRITE_TAC [GEN_ALL can_pmatch_all_IMP_pmatch_rows]
-  \\ rw [] \\ fs []
-  \\ metis_tac [SUBMAP_TRANS, subglobals_trans]
-QED
-
-Triviality compile_correct_Con:
-  ^(#get_goal compile_correct_setup `Case [Con _ _]`)
-Proof
-  rw []
-  \\ fs [pair_case_eq] \\ fs []
-  \\ first_x_assum (drule_then (drule_then drule))
-  \\ disch_then (qspec_then ‘t’ mp_tac)
-  \\ simp []
-  \\ impl_tac >- (CCONTR_TAC \\ fs [])
-  \\ rw []
-  \\ fs [do_con_check_def, opt_case_bool_eq, EXISTS_PROD]
-  >- (
-    (* tuple *)
-    rfs [build_conv_def, compile_exps_reverse, evaluate_def]
-    \\ imp_res_tac result_rel_imp \\ fs [] \\ rveq \\ fs [result_rel_eqns]
-    \\ simp [v_rel_eqns]
-    \\ goal_assum (first_assum o mp_then (Pat `s_rel`) mp_tac)
-    \\ simp []
-  )
-  (* named constructor *)
-  \\ rveq \\ fs [build_conv_def, compile_exps_reverse, evaluate_def]
-  \\ fs [env_all_rel_cases] \\ rveq \\ fs []
-  \\ fs [v_rel_global_eqn]
-  \\ first_x_assum drule
-  \\ rw [EXISTS_PROD]
-  \\ simp [type_group_id_type_MAP, evaluate_def]
-  \\ DEP_REWRITE_TAC [flat_patternProofTheory.COND_true]
-  \\ conj_tac >-
-  (
-    fs [invariant_def, s_rel_cases, FDOM_FLOOKUP, compile_exps_length]
-    \\ rfs []
-  )
-  \\ imp_res_tac result_rel_imp \\ fs [] \\ rveq \\ fs [result_rel_eqns]
-  \\ fs [option_case_eq, pair_case_eq] \\ rveq \\ fs []
-  \\ goal_assum (q_part_match_pat_tac `s_rel _ _ _` mp_tac)
-  \\ simp [v_rel_eqns, result_rel_eqns]
-  \\ imp_res_tac evaluatePropsTheory.evaluate_length
-  \\ fs []
-  \\ metis_tac [FLOOKUP_SUBMAP]
-QED
-
-Triviality compile_correct_Var:
-  ^(#get_goal compile_correct_setup `Case [Var _]`)
-Proof
-  rw []
-  \\ fs [option_case_eq]
-  \\ fs [env_all_rel_cases]
-  \\ rveq \\ fs []
-  \\ fs [nsLookup_nsAppend_some]
-  >- ((* Local variable *)
-    fs [nsLookup_alist_to_ns_some,bind_locals_def] >>
-    rw [] >>
-    drule env_rel_lookup >>
-    disch_then drule >>
-    rw [GSYM nsAppend_to_nsBindList] >>
-    simp[MAP2_MAP]>>
-    every_case_tac >>
-    fs [nsLookup_nsAppend_some, nsLookup_nsAppend_none, nsLookup_alist_to_ns_some,
-        nsLookup_alist_to_ns_none,evaluate_def]>>
-    fs[ALOOKUP_NONE,MAP_MAP_o,o_DEF,LAMBDA_PROD]>>
-    `(λ(p1:tra,p2:tvarN). p2) = SND` by fs[FUN_EQ_THM,FORALL_PROD]>>
-    fs[]>>rfs[MAP_ZIP]
-    >- metis_tac [ALOOKUP_MEM,PAIR,FST,MEM_MAP, SUBMAP_REFL, subglobals_refl]
-    >- metis_tac [ALOOKUP_MEM,PAIR,FST,MEM_MAP, SUBMAP_REFL, subglobals_refl]
-    >- (
-      drule ALOOKUP_MEM >>
-      rw [MEM_MAP] >>
-      pairarg_tac>>fs[compile_var_def]>>
-      simp [evaluate_def, result_rel_cases] >>
-      metis_tac [SUBMAP_REFL, subglobals_refl])
-    >- metis_tac [ALOOKUP_MEM,PAIR,FST,MEM_MAP])
-  >- ( (* top-level variable *)
-    rw [GSYM nsAppend_to_nsBindList,bind_locals_def] >>
-    fs [nsLookup_alist_to_ns_none] >>
-    fs [v_rel_global_eqn, ALOOKUP_NONE, METIS_PROVE [] ``~x ∨ y ⇔ x ⇒ y``] >>
-    first_x_assum drule >>
-    rw [] >>
-    simp[MAP2_MAP]>>
-    every_case_tac >>
-    fs [nsLookup_nsAppend_some, nsLookup_nsAppend_none, nsLookup_alist_to_ns_some,
-        nsLookup_alist_to_ns_none]>>
-    fs[ALOOKUP_NONE,MAP_MAP_o,o_DEF,LAMBDA_PROD]
-    >- (Cases_on`p1`>>fs[])
-    >- (
-      drule ALOOKUP_MEM >>
-      simp[MEM_MAP,MEM_ZIP,EXISTS_PROD]>>
-      rw[]>>
-      metis_tac[MEM_EL,LENGTH_MAP])
-    >- (
-      rfs [ALOOKUP_TABULATE] >>
-      rw [] >>
-      simp [evaluate_def, result_rel_cases,compile_var_def] >>
-      simp [do_app_def] >>
-      imp_res_tac invariant_globals >>
-      fs [] >>
-      metis_tac [subglobals_refl, SUBMAP_REFL]))
-QED
-
-Triviality compile_correct_Fun:
-  ^(#get_goal compile_correct_setup `Case [Fun _ _]`)
-Proof
-  rw [Once v_rel_cases] >>
-  goal_assum (first_assum o mp_then (Pat `invariant`) mp_tac) >>
-  fs [env_all_rel_cases, subglobals_refl] >>
-  srw_tac[][] >>
-  rename [`global_env_inv genv comp_map (set (MAP FST locals)) env`] >>
-  MAP_EVERY qexists_tac [`comp_map`, `env`, `alist_to_ns locals`,`t`,`None::ts`] >>
-  imp_res_tac env_rel_dom >>
-  srw_tac[][] >>
-  simp [bind_locals_def, namespaceTheory.nsBindList_def] >>
-  fs [ADD1]
-  >- metis_tac [sem_env_eq_lemma]
-  >- metis_tac[LENGTH_MAP]
-QED
-
 Theorem v_to_list_SOME_step:
   !v. v_to_list v = SOME xs ==>
   v = Conv (SOME (TypeStamp "[]" list_type_num)) [] /\ xs = []
@@ -3323,7 +2711,8 @@ Theorem src_orac_env_invs_lookup_env:
 Proof
   PairCases_on `env_id`
   \\ rw [lookup_env_def, case_eq_thms]
-  \\ fs [src_orac_invs_def, src_orac_env_invs_def, src_orac_next_cfg_def]
+  \\ fs [src_orac_invs_def, src_orac_env_invs_def, src_orac_next_cfg_def,
+        src_orac_next_cfg_inner_def]
   \\ every_case_tac \\ fs []
   \\ rfs []
   \\ fs [lem_listTheory.list_index_def]
@@ -3360,7 +2749,7 @@ Proof
   \\ pairarg_tac \\ fs []
   \\ rfs []
   \\ fs []
-  \\ simp [src_orac_next_cfg_def]
+  \\ simp [src_orac_next_cfg_def, src_orac_next_cfg_inner_def]
 QED
 
 Theorem subglobals_add_NONE:
@@ -3390,10 +2779,14 @@ Theorem do_eval:
   idx_prev end_idx c'.next /\
   genv.c ⊑ genv'.c /\
   genv.tys ⊑ genv'.tys /\
-  subglobals genv.v genv'.v
-
+  subglobals genv.v genv'.v /\
+  (case s.eval_state of SOME (EvalOracle s) =>
+    ?s'. eval_state = SOME (EvalOracle s') /\
+    s'.envs = (add_env_generation s).envs /\
+    s'.generation = (add_env_generation s).generation
+    | _ => F
+  )
 Proof
-
   rw [semanticPrimitivesTheory.do_eval_def, do_eval_def]
   \\ fs [case_eq_thms, invariant_def]
   \\ rfs [CaseEq "eval_state"] \\ rfs []
@@ -3417,11 +2810,13 @@ Proof
   \\ drule compile_prog_nonempty
   \\ rw []
   \\ asm_exists_tac
-  \\ simp []
+  \\ simp [EVAL ``(add_env_generation s).envs``,
+        EVAL ``(add_env_generation s).generation``]
   \\ qmatch_goalsub_abbrev_tac `src_orac_next_cfg (SOME i_f) (SOME es2) = SOME c1`
   \\ `src_orac_next_cfg (SOME i_f) (SOME es2) = SOME c1`
     by (
-    fs [src_orac_next_cfg_def, markerTheory.Abbrev_def, add_env_generation_def]
+    fs [src_orac_next_cfg_def, markerTheory.Abbrev_def, add_env_generation_def,
+        src_orac_next_cfg_inner_def]
   )
   \\ fs []
   \\ imp_res_tac compile_prog_idx_prev
@@ -3469,7 +2864,7 @@ Proof
   >- (
     fs [markerTheory.Abbrev_def, add_env_generation_def]
     \\ fs [src_orac_env_invs_def]
-    \\ simp [src_orac_next_cfg_def]
+    \\ simp [src_orac_next_cfg_def, src_orac_next_cfg_inner_def]
     \\ imp_res_tac compile_prog_env_submap
     \\ rfs []
     \\ rveq \\ fs []
@@ -3519,15 +2914,629 @@ Proof
   )
 QED
 
+Theorem invariant_end_eval:
+  invariant interp gen' genv (x, end_idx1, idx_block idx end_idx ∪ other) st st' ∧
+  invariant interp gen prev_genv (idx, end_idx, other) prev_st prev_st' ∧
+  orac_forward_rel begin_eval_state st.eval_state ∧
+  idx_prev end_idx end_idx1 ∧
+  (case prev_st.eval_state of SOME (EvalOracle s) =>
+    ?s'. begin_eval_state = SOME (EvalOracle s') ∧
+    s'.envs = (add_env_generation s).envs ∧
+    s'.generation = (add_env_generation s).generation
+    | _ => F
+  )
+  ⇒
+  invariant interp gen genv (idx, end_idx, other) (st with
+        eval_state := reset_env_generation prev_st.eval_state st.eval_state)
+    st' ∧
+  orac_forward_rel prev_st.eval_state
+    (reset_env_generation prev_st.eval_state st.eval_state)
+Proof
+  every_case_tac \\ fs []
+  \\ rw [] \\ fs [invariant_def, src_orac_invs_def]
+  \\ Cases_on `interp`
+  >- (
+    fs [src_orac_step_invs_def, orac_forward_rel_def] \\ fs []
+  )
+  \\ fs [orac_forward_rel_def] \\ fs [reset_env_generation_def]
+  \\ rfs [src_orac_next_cfg_def]
+  \\ rw []
+  \\ TRY (fs [src_orac_env_invs_def, src_orac_step_invs_def, orac_rel_def,
+        src_orac_next_cfg_def, s_rel_cases, fin_idx_match_def]
+    \\ fsrw_tac [SATISFY_ss] []
+    \\ NO_TAC)
+  >- (
+    fs [idx_range_rel_def, src_orac_next_cfg_def]
+    \\ qexists_tac `fin_idx`
+    \\ fsrw_tac [SATISFY_ss] [idx_prev_trans]
+    \\ drule (Q.SPECL [`2`, `0`, `mv_set`, `[_; _; mv_set ∪ other; _]`]
+          ALL_DISJOINT_MOVE)
+    \\ rw [LUPDATE_compute]
+    \\ drule_then irule ALL_DISJOINT_SUBSETS
+    \\ simp [SUBSET_DEF, PULL_EXISTS]
+    \\ imp_res_tac (Q.SPECL [`x`, `2`] ALL_DISJOINT_elem)
+    \\ fs []
+  )
+  >- (
+    fs [env_gen_rel_def, add_env_generation_def]
+    \\ simp [EL_APPEND_IF]
+  )
+  >- (
+    fs [add_env_generation_def]
+  )
+  >- (
+    fs [add_env_generation_def]
+    \\ fs [env_gen_rel_def, EL_APPEND_IF]
+  )
+QED
 
-Theorem invariant_reset_env_generation:
+Theorem alloc_tags1_imp:
+  ! ctors ns spt tag_list.
+  alloc_tags1 ctors = (ns, spt, tag_list) ∧
+  ALL_DISTINCT (MAP FST ctors) ==>
+  ? cn_tags.
+  ns = alist_to_ns (MAP (\(cn, tag, arity). (cn, tag)) cn_tags) ∧
+  set (MAP SND cn_tags) = {(tag, arity) |
+    ∃max. lookup arity spt = SOME max ∧ tag < max} ∧
+  tag_list = MAP SND cn_tags ∧
+  ALL_DISTINCT tag_list ∧
+  LIST_REL (\(cn, ts) (cn', _, arity). cn = cn' ∧ arity = LENGTH ts)
+    ctors cn_tags ∧
+  MAP FST ctors = MAP FST cn_tags
+Proof
+  ho_match_mp_tac alloc_tags1_ind
+  \\ simp [alloc_tags1_def]
+  \\ rw []
+  \\ rpt (pairarg_tac \\ fs [])
+  \\ rveq \\ fs []
+  \\ simp [PULL_EXISTS, EXISTS_PROD, lookup_def]
+  \\ qexists_tac `cn_tags`
+  \\ fs [lookup_inc_def, option_case_eq] \\ rveq \\ fs []
+  \\ simp [EVERY_MEM, MEM_MAP, FORALL_PROD, EXISTS_PROD]
+  \\ simp [lookup_insert, EXTENSION]
+  \\ rw [] \\ EQ_TAC \\ rw []
+  \\ rw [] \\ fs []
+  \\ fs [bool_case_eq, Q.ISPEC `SOME v` EQ_SYM_EQ]
+QED
 
-invariant interp gen genv' (idx,end_idx,other)
-              (st2 with
-               eval_state :=
-                 reset_env_generation st'.eval_state st2.eval_state) s1_i1
+(* FIXME also in flat_pattern *)
+Theorem ALOOKUP_MAP_3:
+  (!x. MEM x xs ==> FST (f x) = FST x) ==>
+  ALOOKUP (MAP f xs) x = OPTION_MAP (\y. SND (f (x, y))) (ALOOKUP xs x)
+Proof
+  Induct_on `xs` \\ rw []
+  \\ fs [DISJ_IMP_THM, FORALL_AND_THM]
+  \\ Cases_on `f h`
+  \\ Cases_on `h`
+  \\ rw []
+  \\ fs []
+QED
 
+Theorem alloc_tags_invariant:
+  alloc_tags idx.tidx (ctors : (string # ast_t list) list) = (ns, cids) ∧
+  invariant interp gen genv (idx, end_idx, os) st st' ∧
+  global_env_inv genv comp_map {} env ∧
+  ALL_DISTINCT (MAP FST ctors) ∧
+  idx.tidx + 1 <= end_idx.tidx
+  ⇒
+  ?genv'.
+  genv.c ⊑ genv'.c ∧
+  genv.tys ⊑ genv'.tys ∧
+  genv'.v = genv.v ∧
+  invariant interp gen genv' (idx with tidx := idx.tidx + 1, end_idx, os)
+    (st with next_type_stamp := st.next_type_stamp + 1)
+    (st' with c updated_by $UNION {((idx',SOME idx.tidx),arity) |
+                       (∃max. lookup arity cids = SOME max ∧ idx' < max)}) ∧
+  (let build_env = <| c := alist_to_ns
+        (REVERSE (build_constrs st.next_type_stamp ctors)); v := nsEmpty |> in
+   global_env_inv genv' <| c := ns; v := nsEmpty |> {} build_env ∧
+   env_domain_eq <|c := ns; v := nsEmpty|> build_env)
+Proof
+  rw [invariant_def]
+  \\ fs [s_rel_cases]
+  \\ fs [alloc_tags_def]
+  \\ rpt (pairarg_tac \\ fs [])
+  \\ rveq \\ fs []
+  \\ Cases_on `ctors = []`
+  >- (
+    fs [alloc_tags1_def] \\ rveq \\ fs []
+    \\ qexists_tac `genv`
+    \\ simp [lookup_def, build_constrs_def, v_rel_cases, env_domain_eq_def]
+    \\ fs [idx_range_rel_def]
+    \\ asm_exists_tac
+    \\ simp []
+    \\ drule_then irule ALL_DISJOINT_SUBSETS
+    \\ simp []
+    \\ simp [SUBSET_DEF, idx_block_def]
+    \\ rw []
+  )
+  \\ drule alloc_tags1_imp
+  \\ rw []
+  \\ qexists_tac `genv with <| c := FUNION genv.c (alist_to_fmap
+        (MAP (\(cn, tag, arity). (((tag, SOME idx.tidx), arity),
+            TypeStamp cn st.next_type_stamp)) cn_tags));
+        tys := FUNION genv.tys (alist_to_fmap [(idx.tidx, MAP SND cn_tags)])
+    |>`
+  \\ rw [SUBMAP_FUNION_ID]
+  >- (
+    drule_then irule genv_c_ok_extend
+    \\ rw [FORALL_PROD]
+    \\ imp_res_tac ALOOKUP_MEM
+    \\ fs [MEM_MAP, EXISTS_PROD] \\ rveq \\ fs []
+    \\ simp [same_type_def, ctor_same_type_def]
+    \\ rveq \\ fs []
+    \\ imp_res_tac alistTheory.ALOOKUP_ALL_DISTINCT_MEM
+    \\ fs []
+    \\ TRY strip_tac
+    \\ rveq \\ fs []
+    \\ fs [idx_range_rel_def]
+    \\ rfs [FRANGE_FLOOKUP]
+    \\ qspecl_then [`(i,Idx_Type)`, `0`] drule ALL_DISJOINT_elem
+    \\ simp [idx_block_def]
+    \\ qexists_tac `idx.tidx`
+    \\ simp [FDOM_FLOOKUP]
+    \\ metis_tac []
+  )
+  >- (
+    irule genv_c_tys_ok_extend
+    \\ simp [genv_c_tys_ok_def]
+    \\ conj_tac
+    >- (
+      fs [idx_range_rel_def, genv_c_tys_ok_def]
+      \\ qspecl_then [`(i,Idx_Type)`, `0`] drule ALL_DISJOINT_elem
+      \\ simp []
+      \\ disch_then (qspec_then `idx.tidx` mp_tac)
+      \\ simp [idx_block_def]
+    )
+    \\ simp [genv_c_tys_ok_def, MEM_MAP, EXISTS_PROD, PULL_EXISTS]
+    \\ simp [FLOOKUP_UPDATE, MEM_MAP, EXISTS_PROD]
+    \\ metis_tac []
+  )
+  >- (
+    drule_then irule LIST_REL_sv_rel_weak
+    \\ simp [subglobals_refl, SUBMAP_FUNION_ID]
+  )
+  >- (
+    fs [EXTENSION, FORALL_PROD, MEM_MAP, EXISTS_PROD]
+    \\ metis_tac []
+  )
+  >- (
+    fs [idx_range_rel_def]
+    \\ asm_exists_tac
+    \\ rw []
+    \\ fs [FRANGE_FLOOKUP, FLOOKUP_FUNION, option_case_eq, FLOOKUP_UPDATE]
+    \\ TRY (CCONTR_TAC \\ fs [] \\ imp_res_tac ALOOKUP_MEM
+      \\ fs [MEM_MAP, EXISTS_PROD] \\ NO_TAC)
+    \\ drule_then irule (Q.SPECL [`0`, `3`] ALL_DISJOINT_MOVE)
+    \\ simp [LUPDATE_compute]
+    \\ qexists_tac `{(idx.tidx, Idx_Type)}`
+    \\ simp [EXTENSION, FORALL_PROD, idx_types_FORALL, idx_block_def]
+    \\ simp [MEM_MAP, EXISTS_PROD, PULL_EXISTS]
+    \\ rw [] \\ EQ_TAC \\ rw []
+    \\ fs [NOT_NIL_EQ_LENGTH_NOT_0, quantHeuristicsTheory.LIST_LENGTH_2]
+    \\ rveq \\ fs [EXISTS_PROD]
+    \\ metis_tac []
+  )
+  >- (
+    drule_then irule src_orac_invs_weak
+    \\ simp [subglobals_refl, SUBMAP_FUNION_ID]
+  )
+  >- (
+    simp [build_constrs_def]
+    \\ simp [Once v_rel_cases]
+    \\ rw [nsLookup_alist_to_ns_some]
+    \\ imp_res_tac ALOOKUP_MEM
+    \\ fs [MEM_MAP, EXISTS_PROD] \\ rveq \\ fs []
+    \\ simp [MAP_MAP_o, o_DEF, ELIM_UNCURRY]
+    \\ drule_then drule LIST_REL_MEM_IMP
+    \\ rw [EXISTS_PROD]
+    \\ imp_res_tac alistTheory.ALOOKUP_ALL_DISTINCT_MEM
+    \\ simp [ALOOKUP_MAP_3, FLOOKUP_FUNION]
+    \\ simp [option_case_eq, ALOOKUP_MAP_3]
+    \\ rfs [idx_range_rel_def, FLOOKUP_UPDATE]
+    \\ qspecl_then [`(i,Idx_Type)`, `0`] drule ALL_DISJOINT_elem
+    \\ simp []
+    \\ disch_then (qspec_then `idx.tidx` mp_tac)
+    \\ simp [idx_block_def, flookup_thm]
+    \\ rw []
+    \\ irule alistTheory.ALOOKUP_ALL_DISTINCT_MEM
+    \\ simp [MEM_MAP, EXISTS_PROD]
+    \\ simp [MAP_MAP_o, o_DEF]
+    \\ simp [GSYM MAP_MAP_o |> REWRITE_RULE [o_DEF] |> Q.SPEC `f`
+                |> Q.ISPEC `SND`]
+    \\ irule ALL_DISTINCT_MAP_INJ
+    \\ simp [FORALL_PROD]
+  )
+  >- (
+    simp [env_domain_eq_def]
+    \\ simp [MAP_MAP_o, o_DEF, build_constrs_def, MAP_REVERSE, ELIM_UNCURRY]
+    \\ simp [GSYM MAP_MAP_o |> REWRITE_RULE [o_DEF] |> Q.SPEC `f`
+                |> Q.ISPEC `FST`]
+  )
+QED
 
+val nsAppend_foldl' = Q.prove (
+  `!l ns ns'.
+   nsAppend (FOLDL (λns (l,cids). nsAppend l ns) ns' l) ns
+   =
+   FOLDL (λns (l,cids). nsAppend l ns) (nsAppend ns' ns) l`,
+  Induct_on `l` >>
+  rw [] >>
+  PairCases_on `h` >>
+  rw []);
+
+val nsAppend_foldl = Q.prove (
+  `!l ns.
+   FOLDL (λns (l,cids). nsAppend l ns) ns l
+   =
+   nsAppend (FOLDL (λns (l,cids). nsAppend l ns) nsEmpty l) ns`,
+  metis_tac [nsAppend_foldl', nsAppend_nsEmpty]);
+
+val build_tdefs_no_mod = Q.prove (
+  `!idx tdefs. nsDomMod (build_tdefs idx tdefs) = {[]}`,
+  Induct_on `tdefs` >>
+  rw [build_tdefs_def] >>
+  PairCases_on `h` >>
+  rw [build_tdefs_def] >>
+  pop_assum (qspec_then `idx+1` mp_tac) >>
+  rw [nsDomMod_nsAppend_flat]);
+
+val extend_env_v_empty =
+``extend_env <| c := c; v := nsEmpty |> <| c := c'; v := nsEmpty |>``
+  |> SIMP_CONV (srw_ss ()) [extend_env_def]
+
+val extend_dec_env_v_empty =
+``extend_dec_env <| c := c; v := nsEmpty |> <| c := c'; v := nsEmpty |>``
+  |> SIMP_CONV (srw_ss ()) [extend_dec_env_def]
+
+Theorem nsLookup_nsBind_If:
+  nsLookup (nsBind n v e) nm = (if nm = Short n then SOME v else nsLookup e nm)
+Proof
+  Cases_on `e`
+  \\ Cases_on `nm`
+  \\ simp [namespaceTheory.nsBind_def, namespaceTheory.nsLookup_def]
+  \\ simp [EQ_SYM_EQ]
+QED
+
+Theorem invariant_IMP_s_rel:
+  invariant interp gen genv idx st st' ==> s_rel genv st st'
+Proof
+  simp [invariant_def]
+QED
+
+Theorem invariant_to_st_refs:
+  invariant interp gen genv idx st st' ==>
+  LIST_REL (sv_rel genv) st.refs st'.refs
+Proof
+  simp [invariant_def, s_rel_cases]
+QED
+
+Definition abort_def:
+  abort r <=> (case r of Rerr (Rabort a) => T
+    | _ => F)
+End
+
+Triviality not_abort_IMP_cases:
+  (~ abort r ==> P) ==>
+  ((?a. r = Rerr (Rabort a)) \/ (~ abort r /\ P))
+Proof
+  simp [abort_def] \\ every_case_tac \\ simp []
+QED
+
+Theorem abort_simps[simp]:
+  abort (Rerr (Rabort a)) = T /\
+  abort (Rerr (Rraise e)) = F /\
+  abort (Rval v) = F
+Proof
+  simp [abort_def]
+QED
+
+Definition Case_def:
+  Case X <=> T
+End
+
+Theorem elim_Case:
+  (Case X /\ Y) = Y /\
+  (Case X ==> Y) = Y
+Proof
+  simp [Case_def]
+QED
+
+fun is_app_case t = is_comb t andalso same_const ``Case`` (rator t)
+
+fun setup (q : term quotation, t : tactic) = let
+    val the_concl = Parse.typedTerm q bool
+    val t2 = (t \\ rpt (pop_assum mp_tac))
+    val (goals, validation) = t2 ([], the_concl)
+    fun get_goal q = first (can (rename [q])) goals |> snd
+    fun init thms st = if null (fst st) andalso aconv (snd st) the_concl
+      then ((K (goals, validation)) \\ TRY (MAP_FIRST ACCEPT_TAC thms)) st
+      else failwith "setup tactic: mismatching starting state"
+    val cases = map (find_terms is_app_case o snd) goals
+  in {get_goal = get_goal, concl = fn () => the_concl,
+    cases = cases, init = (init : thm list -> tactic),
+    all_goals = fn () => map snd goals} end
+
+val compile_correct_setup = setup (`
+  (∀ ^s env es s' r genv comp_map env_i1 ^s_i1 es_i1 locals t ts gen idxs.
+    evaluate$evaluate s env es = (s', r) ∧
+    Case es ∧
+    invariant interp gen genv idxs s s_i1 ∧
+    env_all_rel genv comp_map env env_i1 locals ∧
+    LENGTH ts = LENGTH locals ∧
+    r ≠ Rerr (Rabort Rtype_error) ∧
+    es_i1 = compile_exps t (comp_map with v := bind_locals ts locals comp_map.v) es
+    ⇒
+    ?s'_i1 r_i1 genv'.
+    flatSem$evaluate env_i1 s_i1 es_i1 = (s'_i1, r_i1) ∧
+    result_rel (LIST_REL o v_rel) genv' r r_i1 ∧
+    s_rel genv' s' s'_i1 ∧
+    (~ abort r ⇒
+      invariant interp gen genv' idxs s' s'_i1 ∧
+      orac_forward_rel s.eval_state s'.eval_state ∧
+      genv.c ⊑ genv'.c ∧
+      genv.tys ⊑ genv'.tys ∧
+      subglobals genv.v genv'.v)
+  ) ∧
+  (∀ ^s env v pes err_v genv comp_map s' r env_i1 ^s_i1 v_i1 pes_i1
+         err_v_i1 locals t ts gen idxs.
+    evaluate$evaluate_match s env v pes err_v = (s', r) ∧
+    Case pes ∧
+    invariant interp gen genv idxs s s_i1 ∧
+    env_all_rel genv comp_map env env_i1 locals ∧
+    v_rel genv v v_i1 ∧
+    LENGTH ts = LENGTH locals ∧
+    r ≠ Rerr (Rabort Rtype_error) ∧
+    pes_i1 = compile_pes t (comp_map with v := bind_locals ts locals comp_map.v) pes ∧
+    pmatch_rows pes_i1 s_i1 v_i1 <> Match_type_error ∧
+    v_rel genv err_v err_v_i1
+    ⇒
+    ?s'_i1 r_i1 genv'.
+    flatProps$evaluate_match env_i1 s_i1 v_i1 pes_i1 err_v_i1 = (s'_i1, r_i1) ∧
+    result_rel (LIST_REL o v_rel) genv' r r_i1 ∧
+    s_rel genv' s' s'_i1 ∧
+    (~ abort r ⇒
+      invariant interp gen genv' idxs s' s'_i1 ∧
+      orac_forward_rel s.eval_state s'.eval_state ∧
+      genv.c ⊑ genv'.c ∧
+      genv.tys ⊑ genv'.tys ∧
+      subglobals genv.v genv'.v)
+  ) ∧
+  (∀ ^s env ds s' r path t idx end_idx os comp_map ^s_i1 idx'
+        comp_map' ds_i1 t' genv gen gen'.
+    evaluate$evaluate_decs s env ds = (s',r) ∧
+    Case ds ∧
+    invariant interp gen genv (idx, end_idx, os) s s_i1 ∧
+    source_to_flat$compile_decs path t idx comp_map gen ds =
+        (t', idx', comp_map', gen', ds_i1) ∧
+    env_gen_end_rel gen' interp s.eval_state ∧
+    r ≠ Rerr (Rabort Rtype_error) ∧
+    global_env_inv genv comp_map {} env ∧
+    idx_prev idx' end_idx
+    ⇒
+    ? ^s1_i1 genv' r_i1.
+    flatSem$evaluate_decs s_i1 ds_i1 = (s1_i1,r_i1) ∧
+    s_rel genv' s' s1_i1 ∧
+    (~ abort r ⇒
+      invariant interp gen' genv' (idx', end_idx, os) s' s1_i1 ∧
+      orac_forward_rel s.eval_state s'.eval_state ∧
+      genv.c ⊑ genv'.c ∧
+      genv.tys ⊑ genv'.tys ∧
+      subglobals genv.v genv'.v
+    ) ∧
+    (!env'.
+      r = Rval env'
+      ⇒
+      r_i1 = NONE ∧
+      env_domain_eq comp_map' env' ∧
+      global_env_inv genv' comp_map' {} env') ∧
+    (!err.
+      r = Rerr err
+      ⇒
+      ?err_i1.
+        r_i1 = SOME err_i1 ∧
+        result_rel (\a b (c:'a). T) genv' (Rerr err) (Rerr err_i1))
+  )
+  `,
+  ho_match_mp_tac terminationTheory.full_evaluate_ind
+  \\ rw [terminationTheory.full_evaluate_def, flat_evaluate_def,
+    compile_exp_def, compile_decs_def]
+  \\ imp_res_tac invariant_IMP_s_rel
+  \\ fs [result_rel_eqns, v_rel_eqns_non_global, elim_Case]
+)
+
+(*
+  #all_goals compile_correct_setup ()
+*)
+
+val trans_thms = [SUBMAP_TRANS, SUBSET_TRANS,
+    subglobals_trans, orac_forward_rel_trans]
+
+Triviality compile_correct_seq:
+  ^(#get_goal compile_correct_setup `Case (_ :: _ :: _)`)
+Proof
+  rw []
+  \\ fs [pair_case_eq] \\ fs []
+  \\ first_x_assum (drule_then (drule_then drule))
+  \\ disch_then (qspec_then ‘t’ mp_tac)
+  \\ reverse (fs [result_case_eq])
+  >- (
+    rw []
+    \\ fs [result_rel_cases]
+    \\ asm_exists_tac \\ simp []
+  )
+  \\ fs [pair_case_eq]
+  \\ rveq \\ fs []
+  \\ rw []
+  \\ fs [result_rel_cases]
+  \\ rveq \\ fs []
+  \\ drule_then drule env_all_rel_weak
+  \\ rw []
+  \\ first_x_assum (drule_then (drule_then drule))
+  \\ disch_then (qspec_then ‘t’ mp_tac)
+  \\ simp []
+  \\ impl_tac >- (CCONTR_TAC >> fs [])
+  \\ imp_res_tac evaluate_sing \\ fs [] \\ rveq \\ fs []
+  \\ rw [] \\ fs [] \\ rveq \\ fs []
+  \\ metis_tac (v_rel_weak :: trans_thms)
+QED
+
+Triviality compile_correct_Raise:
+  ^(#get_goal compile_correct_setup `Case [Raise _]`)
+Proof
+  rw []
+  \\ fs [pair_case_eq]
+  \\ rveq \\ fs []
+  \\ first_x_assum (drule_then (drule_then drule))
+  \\ disch_then (qspec_then ‘t’ mp_tac)
+  \\ simp []
+  \\ impl_tac >- (CCONTR_TAC \\ fs [])
+  \\ rw []
+  \\ fs [result_rel_cases] \\ rveq \\ fs [] \\ rveq \\ fs []
+  \\ imp_res_tac evaluatePropsTheory.evaluate_sing
+  \\ imp_res_tac evaluate_sing
+  \\ rveq \\ fs []
+  \\ asm_exists_tac \\ simp []
+QED
+
+Triviality compile_correct_Handle:
+  ^(#get_goal compile_correct_setup `Case [Handle _ _]`)
+Proof
+  rw []
+  \\ fs [pair_case_eq] \\ fs []
+  \\ first_x_assum (drule_then (drule_then drule))
+  \\ disch_then (qspec_then ‘t’ mp_tac)
+  \\ simp []
+  \\ impl_tac >- (CCONTR_TAC \\ fs [])
+  \\ rw []
+  \\ imp_res_tac result_rel_imp \\ fs [] \\ rveq \\ fs []
+  \\ TRY (asm_exists_tac \\ simp [])
+  \\ fs [bool_case_eq, Q.ISPEC `(a, b)` EQ_SYM_EQ]
+  \\ drule_then drule env_all_rel_weak
+  \\ rw []
+  \\ first_x_assum (drule_then drule)
+  \\ rpt (disch_then drule)
+  \\ disch_then (first_assum o mp_then (Pat `v_rel`) mp_tac)
+  \\ disch_then (qspec_then ‘t’ mp_tac)
+  \\ DEP_REWRITE_TAC [GEN_ALL can_pmatch_all_IMP_pmatch_rows]
+  \\ rw [] \\ fs []
+  \\ metis_tac trans_thms
+QED
+
+Triviality compile_correct_Con:
+  ^(#get_goal compile_correct_setup `Case [Con _ _]`)
+Proof
+  rw []
+  \\ fs [pair_case_eq] \\ fs []
+  \\ first_x_assum (drule_then (drule_then drule))
+  \\ disch_then (qspec_then ‘t’ mp_tac)
+  \\ simp []
+  \\ impl_tac >- (CCONTR_TAC \\ fs [])
+  \\ rw []
+  \\ fs [do_con_check_def, opt_case_bool_eq, EXISTS_PROD]
+  >- (
+    (* tuple *)
+    rfs [build_conv_def, compile_exps_reverse, evaluate_def]
+    \\ imp_res_tac result_rel_imp \\ fs [] \\ rveq \\ fs [result_rel_eqns]
+    \\ simp [v_rel_eqns]
+    \\ goal_assum (first_assum o mp_then (Pat `s_rel`) mp_tac)
+    \\ simp []
+  )
+  (* named constructor *)
+  \\ rveq \\ fs [build_conv_def, compile_exps_reverse, evaluate_def]
+  \\ fs [env_all_rel_cases] \\ rveq \\ fs []
+  \\ fs [v_rel_global_eqn]
+  \\ first_x_assum drule
+  \\ rw [EXISTS_PROD]
+  \\ simp [type_group_id_type_MAP, evaluate_def]
+  \\ DEP_REWRITE_TAC [flat_patternProofTheory.COND_true]
+  \\ conj_tac >-
+  (
+    fs [invariant_def, s_rel_cases, FDOM_FLOOKUP, compile_exps_length]
+    \\ rfs []
+  )
+  \\ imp_res_tac result_rel_imp \\ fs [] \\ rveq \\ fs [result_rel_eqns]
+  \\ fs [option_case_eq, pair_case_eq] \\ rveq \\ fs []
+  \\ goal_assum (q_part_match_pat_tac `s_rel _ _ _` mp_tac)
+  \\ simp [v_rel_eqns, result_rel_eqns]
+  \\ imp_res_tac evaluatePropsTheory.evaluate_length
+  \\ fs []
+  \\ metis_tac [FLOOKUP_SUBMAP]
+QED
+
+Triviality compile_correct_Var:
+  ^(#get_goal compile_correct_setup `Case [Var _]`)
+Proof
+  rw []
+  \\ fs [option_case_eq]
+  \\ fs [env_all_rel_cases]
+  \\ rveq \\ fs []
+  \\ fs [nsLookup_nsAppend_some]
+  >- ((* Local variable *)
+    fs [nsLookup_alist_to_ns_some,bind_locals_def] >>
+    rw [] >>
+    drule env_rel_lookup >>
+    disch_then drule >>
+    rw [GSYM nsAppend_to_nsBindList] >>
+    simp[MAP2_MAP]>>
+    every_case_tac >>
+    fs [nsLookup_nsAppend_some, nsLookup_nsAppend_none, nsLookup_alist_to_ns_some,
+        nsLookup_alist_to_ns_none,evaluate_def]>>
+    fs[ALOOKUP_NONE,MAP_MAP_o,o_DEF,LAMBDA_PROD]>>
+    `(λ(p1:tra,p2:tvarN). p2) = SND` by fs[FUN_EQ_THM,FORALL_PROD]>>
+    fs[]>>rfs[MAP_ZIP]
+    >- metis_tac [ALOOKUP_MEM,PAIR,FST,MEM_MAP, SUBMAP_REFL, subglobals_refl]
+    >- metis_tac [ALOOKUP_MEM,PAIR,FST,MEM_MAP, SUBMAP_REFL, subglobals_refl]
+    >- (
+      drule ALOOKUP_MEM >>
+      rw [MEM_MAP] >>
+      pairarg_tac>>fs[compile_var_def]>>
+      simp [evaluate_def, result_rel_cases] >>
+      metis_tac [SUBMAP_REFL, subglobals_refl])
+    >- metis_tac [ALOOKUP_MEM,PAIR,FST,MEM_MAP])
+  >- ( (* top-level variable *)
+    rw [GSYM nsAppend_to_nsBindList,bind_locals_def] >>
+    fs [nsLookup_alist_to_ns_none] >>
+    fs [v_rel_global_eqn, ALOOKUP_NONE, METIS_PROVE [] ``~x ∨ y ⇔ x ⇒ y``] >>
+    first_x_assum drule >>
+    rw [] >>
+    simp[MAP2_MAP]>>
+    every_case_tac >>
+    fs [nsLookup_nsAppend_some, nsLookup_nsAppend_none, nsLookup_alist_to_ns_some,
+        nsLookup_alist_to_ns_none]>>
+    fs[ALOOKUP_NONE,MAP_MAP_o,o_DEF,LAMBDA_PROD]
+    >- (Cases_on`p1`>>fs[])
+    >- (
+      drule ALOOKUP_MEM >>
+      simp[MEM_MAP,MEM_ZIP,EXISTS_PROD]>>
+      rw[]>>
+      metis_tac[MEM_EL,LENGTH_MAP])
+    >- (
+      rfs [ALOOKUP_TABULATE] >>
+      rw [] >>
+      simp [evaluate_def, result_rel_cases,compile_var_def] >>
+      simp [do_app_def] >>
+      imp_res_tac invariant_globals >>
+      fs [] >>
+      metis_tac [subglobals_refl, SUBMAP_REFL]))
+QED
+
+Triviality compile_correct_Fun:
+  ^(#get_goal compile_correct_setup `Case [Fun _ _]`)
+Proof
+  rw [Once v_rel_cases] >>
+  goal_assum (first_assum o mp_then (Pat `invariant`) mp_tac) >>
+  fs [env_all_rel_cases, subglobals_refl] >>
+  srw_tac[][] >>
+  rename [`global_env_inv genv comp_map (set (MAP FST locals)) env`] >>
+  MAP_EVERY qexists_tac [`comp_map`, `env`, `alist_to_ns locals`,`t`,`None::ts`] >>
+  imp_res_tac env_rel_dom >>
+  srw_tac[][] >>
+  simp [bind_locals_def, namespaceTheory.nsBindList_def] >>
+  fs [ADD1]
+  >- metis_tac [sem_env_eq_lemma]
+  >- metis_tac[LENGTH_MAP]
+QED
 
 (* NOTE TO SELF: can't just compile Eval->Install, because source Eval
    returns info. the tuple that identifies the env. we'll need to stash
@@ -3621,57 +3630,35 @@ Proof
     \\ first_x_assum (q_part_match_pat_tac `compile_decs _ _ _ _ _ _` mp_tac)
     \\ fs [dec_clock_def, evaluateTheory.dec_clock_def]
     \\ rfs []
-    \\ disch_then (q_part_match_pat_tac `invariant _ _ _ _ _` mp_tac)
+    \\ disch_then (q_part_match_pat_tac `invariant _ _ _ _ _ _` mp_tac)
     \\ simp [idx_prev_refl]
-    \\ (impl_tac >- (strip_tac >> fs []))
+    \\ impl_tac >- (
+      rpt strip_tac \\ fs []
+      \\ fs [env_gen_end_rel_def]
+      \\ imp_res_tac compile_decs_generation
+      \\ simp []
+    )
     \\ rw []
     \\ fs []
     \\ drule_then assume_tac not_abort_IMP_cases \\ fs [] \\ fs []
     \\ rveq \\ fs [] \\ fsrw_tac [SATISFY_ss] []
-    \\ drule_then drule invariant_end_eval
+
+    \\ fs [result_case_eq] \\ rveq \\ fs [] \\ rveq \\ fs []
+    \\ rveq \\ fs []
+
+cheat
+
+    \\ drule_then (drule_then drule) invariant_end_eval
     \\ rw []
-    \\ fs [result_case_eq] \\ rveq \\ fs []
-    \\ fs [option_case_eq, pair_case_eq] \\ rveq \\ fs []
-    \\ TRY (goal_assum (q_part_match_pat_tac `invariant _ _ _ _ _` mp_tac))
-    \\ fsrw_tac [SATISFY_ss] [subglobals_trans, SUBMAP_TRANS]
+    \\ goal_assum (q_part_match_pat_tac `invariant _ _ _ _ _` mp_tac)
+    \\ fsrw_tac [SATISFY_ss] [invariant_IMP_s_rel, orac_forward_rel_trans]
+    \\ metis_tac trans_thms
 
     (* issues:
-      - 1: reset_env_generation needs to happen on errors
       - 2: return values are wrong. Eval needs to compile to something
            that fetches the ident of the final env
     *)
 
-cheat
-
-    \\ imp_res_tac invariant_end_eval
-
-
-
-
-    \\ drule invariant_begin_eval
-    \\ fs [dec_clock_def]
-    \\ rename [`compile_decs [] 0 _ _ _ = (_, new_fin_idx, _, _)`]
-    \\ disch_then (qspecl_then [`new_fin_idx`, `new_fin_idx`] mp_tac)
-    \\ imp_res_tac compile_decs_idx_prev
-    \\ rw [idx_prev_refl]
-    \\ last_x_assum (drule_then drule)
-    \\ simp [idx_prev_refl]
-    \\ impl_tac
-    >- (
-      drule_then (fn t => simp [t]) global_env_inv_weak
-      \\ rpt strip_tac \\ fs []
-      \\ fs [eval_idx_match_len_def, idx_prev_def]
-    )
-    \\ rw []
-    \\ simp []
-    \\ drule_then drule invariant_end_eval
-    \\ (impl_tac >- metis_tac [idx_prev_trans])
-    \\ rw []
-    \\ fs [result_case_eq] \\ rveq \\ fs []
-    \\ goal_assum (first_assum o mp_then (Pat `invariant`) mp_tac)
-    \\ imp_res_tac result_rel_imp \\ fs [result_rel_eqns]
-    \\ metis_tac [subglobals_trans, SUBMAP_TRANS, v_rel_environment_to_v,
-          global_env_inv_append, global_env_inv_weak, subglobals_refl]
   ) >>
   fs [bool_case_eq]
   >- (
@@ -3696,7 +3683,7 @@ cheat
     drule_then assume_tac invariant_dec_clock >>
     first_x_assum (drule_then (drule_then drule)) >>
     simp [dec_clock_def] >>
-    metis_tac [SUBMAP_TRANS, subglobals_trans, SUBSET_TRANS]
+    metis_tac (SUBSET_TRANS :: trans_thms)
   ) >>
   fs [Q.ISPEC `(a, b)` EQ_SYM_EQ, option_case_eq, pair_case_eq] >>
   rveq >> fs [] >>
@@ -3735,7 +3722,7 @@ Proof
   rw [] >>
   reverse (fs [result_case_eq]) >> rveq >> fs []
   >- (
-    goal_assum (first_assum o mp_then (Pat `invariant`) mp_tac) >>
+    goal_assum (q_part_match_pat_tac `invariant _ _ _` mp_tac) >>
     fs [result_rel_cases] >> rveq >> fs [] >>
     every_case_tac >>
     simp [evaluate_def]
@@ -3745,7 +3732,7 @@ Proof
   >- (
     rveq >> fs [] >>
     fs [evaluate_def, do_if_def, do_log_def, bool_case_eq] >> rveq >> fs [] >>
-    goal_assum (first_assum o mp_then (Pat `invariant`) mp_tac) >>
+    goal_assum (q_part_match_pat_tac `invariant _ _ _` mp_tac) >>
     fs [invariant_def, v_rel_Bool_eqn, Boolv_11] >>
     drule_then (fn t => simp [t]) evaluate_Bool >>
     simp [result_rel_eqns, v_rel_Bool_eqn]
@@ -3756,10 +3743,10 @@ Proof
   first_x_assum (drule_then (drule_then drule)) >>
   disch_then (qspec_then ‘t’ mp_tac) >>
   rw [] >>
-  goal_assum (first_assum o mp_then (Pat `invariant`) mp_tac) >>
+  goal_assum (q_part_match_pat_tac `invariant _ _ _` mp_tac) >>
   fs [evaluate_def, do_if_def, do_log_def, bool_case_eq] >> rveq >> fs [] >>
   fs [invariant_def, v_rel_Bool_eqn, Boolv_11] >>
-  metis_tac [subglobals_trans, SUBMAP_TRANS]
+  metis_tac trans_thms
 QED
 
 Triviality compile_correct_If:
@@ -3780,11 +3767,11 @@ Proof
   disch_then (qspec_then ‘t’ mp_tac) >>
   rw [] >>
   imp_res_tac evaluatePropsTheory.evaluate_sing >>
-  goal_assum (first_assum o mp_then (Pat `invariant`) mp_tac) >>
+  goal_assum (q_part_match_pat_tac `invariant _ _ _` mp_tac) >>
   fs [semanticPrimitivesTheory.do_if_def, bool_case_eq] >> rveq >> fs [] >>
   fs [invariant_def, do_if_def] >>
   rfs [v_rel_Bool_eqn, Boolv_11] >>
-  metis_tac [subglobals_trans, SUBMAP_TRANS]
+  metis_tac trans_thms
 QED
 
 Triviality compile_correct_Mat:
@@ -3811,7 +3798,7 @@ Proof
   \\ impl_tac >- (fs [invariant_def, v_rel_lems])
   \\ rw []
   \\ simp []
-  \\ metis_tac [SUBMAP_TRANS, subglobals_trans]
+  \\ metis_tac trans_thms
 QED
 
 Triviality compile_correct_Let:
@@ -3838,7 +3825,7 @@ Proof
     \\ rw []
     \\ simp [Q.prove (`env with v updated_by opt_bind NONE x = env`,
           simp [environment_component_equality,libTheory.opt_bind_def] )]
-    \\ metis_tac [SUBMAP_TRANS, subglobals_trans]
+    \\ metis_tac trans_thms
   )
   \\ pop_assum (qspec_then ‘x::t’ strip_assume_tac)
   \\ simp [compile_exp_def, evaluate_def]
@@ -3861,7 +3848,7 @@ Proof
   )
   \\ rw []
   \\ simp []
-  \\ metis_tac [SUBMAP_TRANS, subglobals_trans]
+  \\ metis_tac trans_thms
 QED
 
 Triviality compile_correct_Letrec:
@@ -4393,7 +4380,7 @@ Proof
   imp_res_tac evaluate_decs_append >>
   fs [] >>
   asm_exists_tac >>
-  metis_tac [SUBMAP_TRANS, subglobals_trans, SUBSET_TRANS]
+  metis_tac trans_thms
 QED
 
 Theorem compile_correct:
@@ -4755,12 +4742,6 @@ Proof
   \\ rw[let_none_list_def]
 QED
 
-Theorem compile_env_exp_esgc_free:
-  esgc_free (compile_env_exp n env)
-Proof
-  cheat
-QED
-
 Theorem compile_decs_esgc_free:
    !t n next env decs n1 next1 env1 decs1.
      compile_decs t n next env decs = (n1, next1, env1, decs1)
@@ -4771,8 +4752,7 @@ Proof
   \\ rw [compile_decs_def]
   \\ rpt (pairarg_tac \\ fs [])
   \\ rw []
-  \\ fs [compile_exp_esgc_free, make_varls_esgc_free,
-    compile_env_exp_esgc_free]
+  \\ fs [compile_exp_esgc_free, make_varls_esgc_free]
   \\ fs [EVERY_MAP, EVERY_FILTER, MAP_FILTER]
   \\ simp [EVERY_MEM, MEM_MAPi, PULL_EXISTS, UNCURRY]
 QED
@@ -4854,12 +4834,6 @@ Proof
   Induct \\ fs [SNOC]
 QED
 
-Theorem compile_env_exp_set_globals:
-  set_globals (compile_env_exp n env) = {||}
-Proof
-  cheat
-QED
-
 Theorem compile_decs_elist_globals:
   ∀t n next env ds e f g p.
     compile_decs t n next env ds = (e,f,g,p) ⇒
@@ -4872,7 +4846,7 @@ Proof
   \\ rpt (pairarg_tac \\ fs [])
   \\ rw[compile_exp_esgc_free, EVAL ``COUNT_LIST 0``]
   \\ fs [FILTER_APPEND, Q.ISPEC `num_bindings` ETA_THM]
-  \\ simp [compile_env_exp_set_globals, op_gbag_def, EVAL ``COUNT_LIST 1``]
+  \\ simp [op_gbag_def, EVAL ``COUNT_LIST 1``]
   >- (
     simp [miscTheory.MAPi_enumerate_MAP, FILTER_MAP, o_DEF, ELIM_UNCURRY]
   )
